additional datatype for Reg

ARMv8/ARMv8_Exp.thy
@@ -172,8 +172,8 @@ fun subst\<^sub>g :: "('v,'r) subop \<Rightarrow> 'v \<Rightarrow> ('v,'r) exp \
 fun subst\<^sub>i :: "('v,'r) subop \<Rightarrow> ('v,'r) var \<Rightarrow> ('v,'r) exp \<Rightarrow> ('v,'r) subop"
   where
     "subst\<^sub>i i (Reg r) e = subst\<^sub>r i r e" |
-    "subst\<^sub>i i (Glb g) e = subst\<^sub>g i g e" |
-    "subst\<^sub>i i (Tmp r) e = subst\<^sub>r i r e" 
+    "subst\<^sub>i i (Glb g) e = subst\<^sub>g i g e" 
+(*    "subst\<^sub>i i (Tmp r) e = subst\<^sub>r i r e" *)
     
 
 definition smap1
@@ -283,8 +283,8 @@ next
   show ?case by simp
 qed
 
-(* old version
-lemma ev_subst\<^sub>E [simp]:
+(* old version 
+lemma ev_subst\<^sub>E_old [simp]:
   "ev\<^sub>E m (subst\<^sub>E e r f) = ev\<^sub>E (m (r := (ev\<^sub>E m f))) e"
 proof (induct e)
   case (Exp fn rs)
@@ -470,74 +470,21 @@ lemma [simp]:
   by auto
 
 lemma [simp]:
-  "Glb x \<in> Tmp ` e = False"
-  by auto
-
-lemma [simp]:
   "Reg x \<in> Reg ` e = (x \<in> e)"
   by auto
 
-lemma [simp]:
-  "Tmp x \<in> Tmp ` e = (x \<in> e)"
-  by auto
-
-lemma [simp]:
-  "Tmp x \<in> Reg ` e = False"
-  by auto
-
-lemma [simp]:
-  "Reg x \<in> Tmp ` e = False"
-  by auto
-
-(* special case of lemma subst_rd for Tmp: 
-   rd labels every local variable as Reg which then can't be matched if x =Tmp r *)
-
-lemma  subst_rd_tmp:   (* should this be in simp set? *)
-  assumes "x = Tmp r"
-  shows "rd (subst\<^sub>i \<alpha> x e) = rd \<alpha> - {Reg r} \<union> (if (Reg r) \<in> rd \<alpha> then Reg` deps\<^sub>E e else {})"
-  by (induct \<alpha>; auto simp add:assms)
-
-
-lemma subst_rd [simp]:  (* should this still be in simp set? *)
-  assumes "x = Reg r \<or> x = Glb r"
-  shows "rd (subst\<^sub>i \<alpha> x e) = rd \<alpha> - {x} \<union> (if x \<in> rd \<alpha> then Reg ` deps\<^sub>E e else {})" 
-  apply (cases x; cases \<alpha>) using assms by (auto split: if_splits)
-
-
-lemma subst_rd_Reg [simp]:  (* should this still be in simp set? *)
-  "rd (subst\<^sub>i \<alpha> (Reg x) e) = rd \<alpha> - {(Reg x)} \<union> 
-                  (if (Reg x) \<in> rd \<alpha> then Reg ` deps\<^sub>E e else {})" 
-  apply (cases \<alpha>) by (auto split: if_splits)
-
-lemma subst_rd_Glb [simp]:  (* should this still be in simp set? *)
-  "rd (subst\<^sub>i \<alpha> (Glb x) e) = rd \<alpha> - {(Glb x)} \<union> 
-                  (if (Glb x) \<in> rd \<alpha> then Glb ` deps\<^sub>E e else {})" 
-  apply (cases \<alpha>) apply (auto split: if_splits)
-  oops
-
-(*---- *)
-
+lemma subst_rd [simp]: 
+  "rd (subst\<^sub>i \<alpha> x e) = rd \<alpha> - {x} \<union> (if x \<in> rd \<alpha> then Reg ` deps\<^sub>E e else {})" 
+  apply (cases x; cases \<alpha>) by (auto split: if_splits)
 
 lemma subst_barriers [simp]:
   "barriers (subst\<^sub>i \<alpha> x e) = barriers \<alpha>"
   by (cases \<alpha>; cases x; auto)
 
-(* special case of lemma subst_nop for Tmp  
-   rd labels every local variable as Reg which then can't be matched if x =Tmp r *)
-
-lemma subst_nop_tmp [simp]: (* should this be in simp set? *)
-  assumes "x = Tmp r"
-  shows "(Reg r) \<notin> rd \<beta> \<Longrightarrow> subst\<^sub>i \<beta> x e = \<beta>"
-  unfolding smap1_def using assms
-  apply (cases \<beta>; cases x) by (auto split: if_splits)
-
 lemma subst_nop [simp]:    (* should this still be in simp set? *)
-  assumes "x = Reg r \<or> x = Glb r"
-  shows "x \<notin> rd \<beta> \<Longrightarrow> subst\<^sub>i \<beta> x e = \<beta>"
-  unfolding smap1_def using assms 
-  apply (cases \<beta>; cases x) by (auto split: if_splits)
+ "x \<notin> rd \<beta> \<Longrightarrow> subst\<^sub>i \<beta> x e = \<beta>"
+  unfolding smap1_def apply (cases \<beta>; cases x) by (auto split: if_splits)
 
-(*---- *)
 
 
 lemma finite_rd [intro]:
@@ -546,97 +493,9 @@ lemma finite_rd [intro]:
 
 subsection \<open>smap1 Theories\<close>
 
-lemma help1:
-   "smap1 V (Reg y) (smap1 V (Reg x) \<alpha>) = smap1 V (Reg x) (smap1 V (Reg y) \<alpha>)"
-  unfolding smap1_def by (cases "x=y"; auto split: if_splits)
-
-lemma help2:
-   "smap1 V (Glb y) (smap1 V (Glb x) \<alpha>) = smap1 V (Glb x) (smap1 V (Glb y) \<alpha>)"
-  unfolding smap1_def apply (auto split: if_splits) by (cases \<alpha>; auto) 
-
-
-lemma help3:
-   "smap1 V (Reg y) (smap1 V (Glb x) \<alpha>) = smap1 V (Glb x) (smap1 V (Reg y) \<alpha>)"
-  unfolding smap1_def 
-  using subst\<^sub>r.simps subst\<^sub>g.simps apply simp by (cases \<alpha>; auto)
-
-lemma help4:
-  "smap1 V (Reg y) (smap1 V (Tmp x) \<alpha>) = smap1 V (Tmp x) (smap1 V (Reg y) \<alpha>)"
-proof (cases "x=y")
-  case True
-  then show ?thesis unfolding smap1_def apply simp sorry  (* registers have to be distinguishable *)
-next
-  case False
-  then show ?thesis unfolding smap1_def using subst\<^sub>r.simps subst\<^sub>g.simps by simp
-qed
-
-(* currently not used
-lemma help3:
-   "smap1 V (Tmp y) (smap1 V (Tmp x) \<alpha>) = smap1 V (Tmp x) (smap1 V (Tmp y) \<alpha>)"
-  unfolding smap1_def apply simp using subst\<^sub>r_flip by metis
-*)
-
-lemma help5:
-   "smap1 V (Glb y) (smap1 V x \<alpha>) = smap1 V x (smap1 V (Glb y) \<alpha>)"
-proof (cases x)
-  case (Reg x1)
-  then show ?thesis  using help3 by metis
-next
-  case (Glb x2)
-  then show ?thesis  using help2 by metis
-next
-  case (Tmp x3)
-  then show ?thesis 
-  proof (cases "x= (Glb y)")
-    case True
-    then show ?thesis by simp
-  next
-    case False
-    then show ?thesis unfolding smap1_def 
-      using Tmp apply (auto split: if_splits)
-      by (cases \<alpha>; simp)   
-  qed
-qed
-
-
-lemma help6:
-  "smap1 V (Glb y) (smap1 V (Tmp x) \<alpha>) = smap1 V (Tmp x) (smap1 V (Glb y) \<alpha>)"
- unfolding smap1_def apply (auto split: if_splits) by (cases \<alpha>; simp)   
-
-
-lemma help7:
-  "smap1 V (Tmp y) (smap1 V x \<alpha>) = smap1 V x (smap1 V (Tmp y) \<alpha>)"
-proof (cases x)
-  case (Reg x1)
-  then show ?thesis 
-     proof (cases "x1=y")
-       case True
-       then show ?thesis unfolding smap1_def apply simp using Reg apply simp sorry
-       next
-         case False
-         then show ?thesis unfolding smap1_def using Reg by simp
-       qed
- next
-  case (Glb x2) 
-  then show ?thesis unfolding smap1_def apply simp using help6 
-    by (metis smap1_def subst\<^sub>i.simps(2) subst\<^sub>i.simps(3))
- next
-  case (Tmp x3)
-  then show ?thesis unfolding smap1_def using Tmp apply simp 
-    using subst\<^sub>r_flip by metis
-qed
-
-
 lemma smap1_flip [simp]:
   shows "smap1 V y (smap1 V x \<alpha>) = smap1 V x (smap1 V y \<alpha>)"
-  apply(cases y) apply(cases x) apply(cases "x=y")
-  using smap1_def subst\<^sub>r.simps(1) apply simp
-  using help1 apply metis
-  using help3 apply metis
-  using help4 apply metis
-  using help5 apply metis
-  using help7 by metis
-
+  by(cases \<alpha>; cases y; cases x; cases "x=y"; auto simp add: smap1_def)
 
 lemma smap1_rep [simp]:
   "smap1 V x (smap1 V x \<alpha>) = smap1 V x \<alpha>"
@@ -648,18 +507,7 @@ interpretation cfi: comp_fun_idem "smap1 V"  by (standard) auto
 
 lemma smap1_rd [simp]:
   "rd (smap1 M x \<beta>) = rd \<beta> - ({x} \<inter> dom M)"
-proof (cases x)
-  case (Reg x1)
-  then show ?thesis unfolding smap1_def apply simp sorry 
-next
-  case (Glb x2)
-  then show ?thesis unfolding smap1_def apply (auto split: if_splits) sorry
-next
-  case (Tmp x3)
-  then show ?thesis sorry
-qed
-  
-(*  unfolding smap1_def by (auto split: if_splits) *)
+  unfolding smap1_def by (auto split: if_splits)
 
 lemma smap1_wr [simp]:
   "wr (smap1 M x \<beta>) = wr \<beta>"
@@ -671,7 +519,7 @@ lemma smap1_barriers [simp]:
 
 lemma smap1_nop [simp]:
   "x \<notin> rd \<beta> \<Longrightarrow> smap1 M x \<beta> = \<beta>"
-  unfolding smap1_def apply (auto split: if_splits) sorry
+  unfolding smap1_def by (auto split: if_splits)
 
 lemma smap1_nop2 [simp]:
   "M x = None \<Longrightarrow> smap1 M x \<beta> = \<beta>"
@@ -812,8 +660,7 @@ proof -
   have "?L \<subseteq> ?R"
   proof (clarsimp simp: forall_def, cases "x \<in> V")
     fix M assume d: "dom (M :: ('a, 'b) ARMv8_State.var \<Rightarrow> 'a option) = insert x V" "x \<in> V"
-    hence "smap \<alpha> M = subst\<^sub>i (smap \<alpha> M) x (Val (the (M x)))"
-      by (metis insert_absorb smap1_def smap_rep)  (* by simp *)
+    hence "smap \<alpha> M = subst\<^sub>i (smap \<alpha> M) x (Val (the (M x)))" by simp 
     moreover have "dom M = V" using d by auto
     ultimately show "\<exists>c \<alpha>'. smap \<alpha> M = subst\<^sub>i \<alpha>' x (Val c) \<and> (\<exists>M. \<alpha>' = smap \<alpha> M \<and> dom M = V)"
       by blast
@@ -843,8 +690,7 @@ proof -
         case False
         hence [simp]: "rd \<alpha> - {x} = rd \<alpha>" by auto
         have "x \<notin> rd (smap \<alpha> ?M)" using False by simp
-        then show ?thesis using mx unfolding smap_def 
-          by (metis \<open>rd \<alpha> - {x} = rd \<alpha>\<close> d(1) insertCI smap1_def smap1_nop) (* by simp *)
+        then show ?thesis using mx unfolding smap_def by simp 
       qed
     qed
     moreover have "dom ?M = V" using d by (auto split: if_splits)
@@ -856,7 +702,7 @@ proof -
   proof (clarsimp simp: forall_def, cases "x \<in> V")
     fix M c assume d: "V = dom (M :: ('a, 'b) ARMv8_State.var \<Rightarrow> 'a option)" "x \<in> V" 
     have "dom M = insert x (dom M)" using d by auto
-    moreover have "subst\<^sub>i (smap \<alpha> M) x (Val c) = smap \<alpha> M" using d sorry (* by simp *) 
+    moreover have "subst\<^sub>i (smap \<alpha> M) x (Val c) = smap \<alpha> M" using d by simp  
     ultimately show "\<exists>Ma. subst\<^sub>i (smap \<alpha> M) x (Val c) = smap \<alpha> Ma \<and> dom Ma = insert x (dom M)"
       by blast
   next
@@ -886,10 +732,7 @@ proof -
         case False
         hence [simp]: "rd \<alpha> - {x} = rd \<alpha>" by auto
         have "x \<notin> rd (smap \<alpha> ?M)" using False by simp
-        then show ?thesis using mx unfolding smap_def 
-          by (smt (verit, best) \<open>rd \<alpha> - {x} = rd \<alpha>\<close> 
-                        calculation insertCI option.sel smap1_def smap_def smap_rep)
- (*by simp*)
+        then show ?thesis using mx unfolding smap_def by simp
       qed
     qed
     ultimately show "\<exists>Ma. subst\<^sub>i (smap \<alpha> M) x (Val c) = smap \<alpha> Ma \<and> dom Ma = insert x (dom M)"
@@ -906,7 +749,7 @@ lemma forall_one [simp]:
 lemma forall_nop [simp]:
   assumes "x \<notin> rd \<alpha>" 
   shows "forall (insert x V) \<alpha> = forall V \<alpha>"
-  using assms forall_unfold sorry (* by force *)
+  using assms forall_unfold by force
 
 lemma forallI [intro]:
   "smap \<alpha> M \<in> forall (dom M) \<alpha>"
@@ -942,10 +785,32 @@ lemma upd_more [simp]:
   by (auto simp: upd_def)
 
 lemma st_upd_eq [intro]:
-  "state_rec.more m = state_rec.more m' \<Longrightarrow> \<forall>x. x \<noteq> y \<longrightarrow> st m x = st m' x \<Longrightarrow> m(y :=\<^sub>s e) = m'(y :=\<^sub>s e)"
-  oops
-  (*by (auto simp: upd_def st_upd_def intro!: state_rec.equality)
-*)
+  "state_rec.more m = state_rec.more m' \<Longrightarrow> 
+                    \<forall>x. x \<noteq> y \<longrightarrow> st m x = st m' x \<Longrightarrow> m(y :=\<^sub>s e) = m'(y :=\<^sub>s e)"
+  apply (auto simp: upd_def st_upd_def intro!: state_rec.equality)
+  
+
+
+lemma [simp]:
+  "rg (upd V f m) x = (if Reg x \<in> V then f (Reg x) else rg m x)"
+  unfolding rg_def upd_def
+  by simp
+
+lemma [simp]:
+  "rg (m(aux: f)) = rg m"
+  unfolding rg_def aux_upd_def by simp
+
+(* old version: relies on  deps_ev\<^sub>E *)
+lemma [simp]:
+    "Reg ` deps\<^sub>E e \<subseteq> V \<Longrightarrow> ev\<^sub>E (Base (rg (upd (V \<inter> dom M) (the \<circ> M) m\<^sub>1))) e = 
+                         ev\<^sub>E (Base (rg (upd (dom M) (the \<circ> M) m\<^sub>1))) e"
+  by (rule deps_ev\<^sub>E) auto
+
+lemma [simp]:
+  "Reg ` deps\<^sub>B e \<subseteq> V \<Longrightarrow> ev\<^sub>B (rg (upd (V \<inter> dom M) (the \<circ> M) m\<^sub>1)) e = ev\<^sub>B (rg (upd (dom M) (the \<circ> M) m\<^sub>1)) e"
+  by (rule deps_ev\<^sub>B) auto
+
+
 
 (*
 lemma beh_substi [simp]:
@@ -986,25 +851,6 @@ next
 qed
 *)
 
-lemma [simp]:
-  "rg (upd V f m) x = (if Reg x \<in> V then f (Reg x) else rg m x)"
-  unfolding rg_def upd_def
-  by simp
-
-lemma [simp]:
-  "rg (m(aux: f)) = rg m"
-  unfolding rg_def aux_upd_def by simp
-
-(* old version: relies on  deps_ev\<^sub>E
-lemma [simp]:
-  "Reg ` deps\<^sub>E e \<subseteq> V \<Longrightarrow> ev\<^sub>E (Base (rg (upd (V \<inter> dom M) (the \<circ> M) m\<^sub>1))) e = 
-                         ev\<^sub>E (Base (rg (upd (dom M) (the \<circ> M) m\<^sub>1))) e"
-  by (rule deps_ev\<^sub>E) auto
-
-lemma [simp]:
-  "Reg ` deps\<^sub>B e \<subseteq> V \<Longrightarrow> ev\<^sub>B (rg (upd (V \<inter> dom M) (the \<circ> M) m\<^sub>1)) e = ev\<^sub>B (rg (upd (dom M) (the \<circ> M) m\<^sub>1)) e"
-  by (rule deps_ev\<^sub>B) auto
-*)
 
 
 (*
@@ -1021,6 +867,102 @@ proof -
 
   finally show ?thesis unfolding smap_def .
 qed
+*)
+
+
+
+(* some superceded proofs:
+
+lemma help1:
+   "smap1 V (Reg y) (smap1 V (Reg x) \<alpha>) = smap1 V (Reg x) (smap1 V (Reg y) \<alpha>)"
+  unfolding smap1_def by (cases "x=y"; auto split: if_splits)
+
+lemma help2:
+   "smap1 V (Glb y) (smap1 V (Glb x) \<alpha>) = smap1 V (Glb x) (smap1 V (Glb y) \<alpha>)"
+  unfolding smap1_def apply (auto split: if_splits) by (cases \<alpha>; auto) 
+
+
+lemma help3:
+   "smap1 V (Reg y) (smap1 V (Glb x) \<alpha>) = smap1 V (Glb x) (smap1 V (Reg y) \<alpha>)"
+  unfolding smap1_def 
+  using subst\<^sub>r.simps subst\<^sub>g.simps apply simp by (cases \<alpha>; auto)
+
+lemma help4:
+  "smap1 V (Reg y) (smap1 V (Tmp x) \<alpha>) = smap1 V (Tmp x) (smap1 V (Reg y) \<alpha>)"
+proof (cases "x=y")
+  case True
+  then show ?thesis unfolding smap1_def apply simp sorry  (* registers have to be distinguishable *)
+next
+  case False
+  then show ?thesis unfolding smap1_def using subst\<^sub>r.simps subst\<^sub>g.simps by simp
+qed
+
+(* currently not used
+lemma help3:
+   "smap1 V (Tmp y) (smap1 V (Tmp x) \<alpha>) = smap1 V (Tmp x) (smap1 V (Tmp y) \<alpha>)"
+  unfolding smap1_def apply simp using subst\<^sub>r_flip by metis
+*)
+
+lemma help5:
+   "smap1 V (Glb y) (smap1 V x \<alpha>) = smap1 V x (smap1 V (Glb y) \<alpha>)"
+proof (cases x)
+  case (Reg x1)
+  then show ?thesis  using help3 by metis
+next
+  case (Glb x2)
+  then show ?thesis  using help2 by metis
+next
+  case (Tmp x3)
+  then show ?thesis 
+  proof (cases "x= (Glb y)")
+    case True
+    then show ?thesis by simp
+  next
+    case False
+    then show ?thesis unfolding smap1_def 
+      using Tmp apply (auto split: if_splits)
+      by (cases \<alpha>; simp)   
+  qed
+qed
+
+
+lemma help6:
+  "smap1 V (Glb y) (smap1 V (Tmp x) \<alpha>) = smap1 V (Tmp x) (smap1 V (Glb y) \<alpha>)"
+ unfolding smap1_def apply (auto split: if_splits) by (cases \<alpha>; simp)   
+
+
+lemma help7:
+  "smap1 V (Tmp y) (smap1 V x \<alpha>) = smap1 V x (smap1 V (Tmp y) \<alpha>)"
+proof (cases x)
+  case (Reg x1)
+  then show ?thesis 
+     proof (cases "x1=y")
+       case True
+       then show ?thesis unfolding smap1_def apply simp using Reg apply simp sorry
+       next
+         case False
+         then show ?thesis unfolding smap1_def using Reg by simp
+       qed
+ next
+  case (Glb x2) 
+  then show ?thesis unfolding smap1_def apply simp using help6 
+    by (metis smap1_def subst\<^sub>i.simps(2) subst\<^sub>i.simps(3))
+ next
+  case (Tmp x3)
+  then show ?thesis unfolding smap1_def using Tmp apply simp 
+    using subst\<^sub>r_flip by metis
+qed
+
+
+lemma smap1_flip [simp]:
+  shows "smap1 V y (smap1 V x \<alpha>) = smap1 V x (smap1 V y \<alpha>)"
+  apply(cases y) apply(cases x) apply(cases "x=y")
+  using smap1_def subst\<^sub>r.simps(1) apply simp
+  using help1 apply metis
+  using help3 apply metis
+  using help4 apply metis
+  using help5 apply metis
+  using help7 by metis
 *)
 
 end
